src/ReorderingRw.v
@@ -412,17 +412,24 @@ Proof using.
   { intro F; eapply ext_sb_irr with (x := a).
     rewrite F at 2. apply SIM_ACTS. }
   assert (FIN_LAB : lab G_t' = lab_t).
-  { symmetry. destruct STEP, start_wf; ins. apply pfx. }
+  { symmetry. eapply sub_lab.
+    eapply WCore.wf_g_sub_gc
+    with (X := {|
+      WCore.G := G_t;
+      WCore.GC := G_t';
+      WCore.sc := sc;
+      WCore.cmt := ∅;
+    |}).
+    apply STEP. }
   assert (LABEQ : lab_t = lab_t ∘ mapper ∘ mapper).
   { now rewrite Combinators.compose_assoc,
                 ReordCommon.mapper_mapper_compose,
                 Combinators.compose_id_right. }
   assert (SAME' : E_t' a <-> E_t' b).
-  { destruct STEP. red in add_event. desf.
-    destruct add_event. ins.
-    split; intro HSET.
-    all: apply e_new; apply e_new in HSET.
-    all: unfolder; unfolder in HSET; desf.
+  { destruct STEP. split; intro HSET.
+    all: apply (WCore.cae_e_new add_event).
+    all: apply (WCore.cae_e_new add_event) in HSET.
+    all: ins; unfolder; unfolder in HSET; desf.
     all: now left. }
 
   (* actual proof *)
@@ -440,7 +447,7 @@ Proof using.
   { destruct STEP. red in add_event. desf.
     exists (option_map mapper r), (option_map mapper w),
            (mapper ↑₁ W1), (mapper ↑₁ W2).
-    apply WCore.cfg_add_event_iff_struct_and_props. splits.
+    splits; ins.
     { admit. }
     { replace ∅ with (mapper ↑₁ ∅) by now rewrite set_collect_empty.
       replace e with (mapper e) by now rewrite ReordCommon.mapper_neq.
@@ -460,7 +467,7 @@ Proof using.
       { now apply ReordCommon.mapper_inj. }
       { now apply ReordCommon.mapper_surj. }
       { ins. now rewrite FIN_LAB. }
-      eapply WCore.cfg_add_event_iff_struct_and_props; eauto. }
+      apply PROPS. }
     { admit. (* TODO: traces *) }
     replace ∅ with (mapper ↑₁ ∅) by now rewrite set_collect_empty.
     apply ReordCommon.mapped_G_t_cfg with (X := {|
@@ -513,7 +520,15 @@ Proof using.
   { intro F; eapply ext_sb_irr with (x := a).
     rewrite F at 2. apply SIM_ACTS. }
   assert (FIN_LAB : lab G_t' = lab_t).
-  { symmetry. destruct STEP, start_wf; ins. apply pfx. }
+  { symmetry. eapply sub_lab.
+    eapply WCore.wf_g_sub_gc
+    with (X := {|
+      WCore.G := G_t;
+      WCore.GC := G_t';
+      WCore.sc := sc;
+      WCore.cmt := ∅;
+    |}).
+    apply STEP. }
   assert (LABEQ : lab_t = lab_t ∘ mapper ∘ mapper).
   { now rewrite Combinators.compose_assoc,
                 ReordCommon.mapper_mapper_compose,
@@ -528,13 +543,11 @@ Proof using.
     apply ReordCommon.mapper_inj in F; ins. }
   assert (NINA' : ~E_t' a).
   { intro F'. destruct STEP; ins.
-    red in add_event. desf.
-    apply add_event.(WCore.e_new) in F'.
+    apply (WCore.cae_e_new add_event) in F'.
     ins. destruct F' as [HIN|HEQ]; desf. }
   assert (NINB' : ~E_t' b).
   { intro F'. destruct STEP; ins.
-    red in add_event. desf.
-    apply add_event.(WCore.e_new) in F'.
+    apply (WCore.cae_e_new add_event) in F'.
     ins. destruct F' as [HIN|HEQ]; desf. }
   assert (ANREAD : ~ codom_rel (mapper ↑ rf_t') a).
   { unfolder. intro F. desf.
@@ -542,7 +555,7 @@ Proof using.
                                         (x := y') (y := b) in F.
     all: ins; try now rewrite ReordCommon.mapper_eq_b.
     apply NINB'.
-    apply STEP.(WCore.start_wf).(WCore.wf_gc).(wf_rfE) in F.
+    apply (wf_rfE (WCore.wf_gc (WCore.start_wf STEP))) in F.
     ins. unfolder in F. desf. }
   assert (BNREAD : ~ dom_rel (mapper ↑ rf_t') a).
   { unfolder. intro F. desf.
@@ -550,11 +563,11 @@ Proof using.
                                         (x := x') (y := b) in F.
     all: ins; try now rewrite ReordCommon.mapper_eq_b.
     apply NINB'.
-    apply STEP.(WCore.start_wf).(WCore.wf_gc).(wf_rfE) in F.
+    apply (wf_rfE (WCore.wf_gc (WCore.start_wf STEP))) in F.
     ins. unfolder in F. desf. }
   assert (ACTEQ : E_t' ≡₁ E_t ∪₁ eq e).
-  { destruct STEP. red in add_event. desf.
-    rewrite (WCore.e_new add_event). ins. }
+  { destruct STEP.
+    rewrite (WCore.cae_e_new add_event). ins. }
   (* Actual proof *)
   destruct STEP; ins. red in add_event. desf.
   constructor; ins.
@@ -577,18 +590,18 @@ Proof using.
     eapply rsrw_tid_a_tid_b; eauto. }
   { exists (option_map mapper r), (option_map mapper w),
            (mapper ↑₁ W1), (mapper ↑₁ W2).
-    apply WCore.cfg_add_event_iff_struct_and_props. splits.
+    splits.
     { constructor; ins.
       { rewrite ACTEQ, set_collect_union, set_collect_eq,
                 ReordCommon.mapper_neq; ins. }
       { unfolder. intro F. desf.
-        apply (WCore.e_notin add_event). ins.
+        apply STRUCT. ins.
         rewrite ReordCommon.mapper_neq; ins.
         { intro EQ; subst. apply E_NOT_B.
           now rewrite ReordCommon.mapper_eq_a. }
         intro EQ; subst. apply E_NOT_A.
         now rewrite ReordCommon.mapper_eq_b. }
-      apply add_event. }
+      apply STRUCT. }
     { replace ∅ with (mapper ↑₁ ∅) by now rewrite set_collect_empty.
       replace e with (mapper e) by now rewrite ReordCommon.mapper_neq.
       apply cfg_upd_lab_add_step_props with
@@ -621,7 +634,7 @@ Proof using.
       { now apply ReordCommon.mapper_inj. }
       { now apply ReordCommon.mapper_surj. }
       { ins. now rewrite FIN_LAB. }
-      eapply WCore.cfg_add_event_iff_struct_and_props; eauto. }
+      apply PROPS. }
     { admit. (* traces *) }
     replace ∅ with (mapper ↑₁ ∅); [| now rewrite set_collect_empty].
     apply cfg_upd_lab_wf with (X := {|
@@ -687,16 +700,21 @@ Proof using.
   { eapply rsrw_a_neq_b; eauto. }
   assert (INA' : E_t' a).
   { destruct STEP; ins.
-    red in add_event. desf.
-    apply add_event.(WCore.e_new).
+    apply (WCore.cae_e_new add_event).
     ins. now left. }
   assert (NINB' : ~E_t' b).
   { intro F'. destruct STEP; ins.
-    red in add_event. desf.
-    apply add_event.(WCore.e_new) in F'.
+    apply (WCore.cae_e_new add_event) in F'.
     ins. destruct F' as [HIN|HEQ]; desf. }
   assert (FIN_LAB : lab G_t' = lab_t).
-  { symmetry. destruct STEP, start_wf; ins. apply pfx. }
+  { symmetry. destruct STEP; ins.
+    now apply WCore.wf_g_sub_gc
+    with (X := {|
+      WCore.G := G_t;
+      WCore.GC := G_t';
+      WCore.sc := sc;
+      WCore.cmt := ∅;
+    |}). }
   assert (LABEQ : lab_t' = lab_t' ∘ mapper ∘ mapper).
   { rewrite Combinators.compose_assoc.
     rewrite ReordCommon.mapper_mapper_compose; eauto. }
@@ -720,15 +738,15 @@ Proof using.
     { destruct STEP. constructor; ins.
       { unfold FinThreads.fin_threads. ins.
         apply start_wf. }
-      { now rewrite start_wf.(WCore.cc_ctrl_empty), collect_rel_empty. }
-      { now rewrite start_wf.(WCore.cc_addr_empty), collect_rel_empty. }
-      { now rewrite start_wf.(WCore.cc_data_empty), collect_rel_empty. }
+      { now rewrite (WCore.wf_cc_ctrl_empty start_wf), collect_rel_empty. }
+      { now rewrite (WCore.wf_cc_addr_empty start_wf), collect_rel_empty. }
+      { now rewrite (WCore.wf_cc_data_empty start_wf), collect_rel_empty. }
       { apply exec_add_rf_cont. admit. (* TODO: need weaker lemma *) }
       { apply exec_add_rf_cont. admit. }
       { intros x [[INE | EQA] HINIT]; try now right.
         destruct INE as (x' & INE & HEQ).
         left. exists x'; split; eauto.
-        apply start_wf.(WCore.wf_g_init); split; ins.
+        apply (WCore.wf_g_init start_wf); split; ins.
         erewrite ReordCommon.mapper_inj with (x := x') (y := x)
                                              (a := a) (b := b).
         all: ins.
@@ -736,14 +754,14 @@ Proof using.
         rewrite ReordCommon.mapper_init_actid with (a := a) (b := b).
         all: ins; now apply SIM_ACTS. }
       intros x [EQTID [INE | EQA]]; red in EQTID.
-      { apply start_wf.(WCore.wf_gc_acts); split; ins.
+      { apply (WCore.wf_gc_acts start_wf); split; ins.
         destruct INE as (x' & INE & HEQ).
         rewrite ReordCommon.mapper_neq in HEQ; subst; ins.
         all: intro F'; subst x'; eauto.
         apply B_TID. erewrite rsrw_tid_a_tid_b; eauto.
         rewrite ReordCommon.mapper_eq_a; eauto. }
       subst; exfalso; apply SIM_ACTS.(rsrw_ninit_a _ _ _).
-      apply start_wf.(WCore.wf_gc_acts); split; ins. }
+      apply (WCore.wf_gc_acts start_wf); split; ins. }
     apply cfg_add_event_nctrl_wf_props with (X := {|
       WCore.sc := mapper ↑ sc;
       WCore.G := exec_upd_lab _ a l;
@@ -766,8 +784,8 @@ Proof using.
                                           (a := a) (b := b).
       all: ins; try now rewrite ReordCommon.mapper_eq_b.
       destruct STEP.
-      apply start_wf.(WCore.wf_gc).(wf_rfE) in DOM1. ins.
-      unfolder in DOM1; desf. }
+      apply (wf_rfE (WCore.wf_gc start_wf)) in DOM1.
+      ins. unfolder in DOM1; desf. }
     { unfolder. ins. desf. }
     { unfolder. ins. desf. }
     { unfolder. splits; ins; desf.
@@ -788,7 +806,7 @@ Proof using.
       { apply SIM_ACTS. }
       { unfold compose. now rewrite ReordCommon.mapper_eq_a. }
       { unfolder. intro F. desf.
-        apply STEP.(WCore.start_wf).(WCore.wf_gc).(wf_rfE) in F.
+        apply (wf_rfE (WCore.wf_gc (WCore.start_wf STEP))) in F.
         ins. unfolder in F. desf.
         apply NINB'.
         rewrite ReordCommon.mapper_inj with (a := a) (b := b)
@@ -796,7 +814,7 @@ Proof using.
         all: ins.
         now rewrite ReordCommon.mapper_eq_b. }
       { unfolder. intro F. desf.
-        apply STEP.(WCore.start_wf).(WCore.wf_gc).(wf_rfE) in F.
+        apply (wf_rfE (WCore.wf_gc (WCore.start_wf STEP))) in F.
         ins. unfolder in F. desf.
         apply NINB'.
         rewrite ReordCommon.mapper_inj with (a := a) (b := b)
@@ -826,9 +844,8 @@ Proof using.
         apply STEP. }
       (* FIXME: uses auto gen names *)
       { admit. (* TODO: lemma *) }
-      { admit. }
-      apply WCore.wf_iff_struct_and_props, STEP. }
-    { rewrite STEP.(WCore.start_wf).(WCore.cc_ctrl_empty).
+       admit. }
+    { rewrite (WCore.wf_cc_ctrl_empty (WCore.start_wf STEP)).
       now rewrite collect_rel_empty. }
     admit. (* TODO *) }
   { replace ∅ with (mapper ↑₁ ∅) by now rewrite set_collect_empty.
@@ -836,7 +853,7 @@ Proof using.
     destruct STEP. red in add_event. desf. ins.
     exists (option_map mapper r), (option_map mapper w),
            (mapper ↑₁ W1), (mapper ↑₁ W2).
-    apply WCore.cfg_add_event_iff_struct_and_props. splits.
+    splits.
     { admit. }
     { apply cfg_add_event_nctrl_add_step_props with
         (X := {|
@@ -883,29 +900,29 @@ Proof using.
       { now apply ReordCommon.mapper_inj. }
       { now apply ReordCommon.mapper_surj. }
       { ins. }
-      eapply WCore.cfg_add_event_iff_struct_and_props; eauto. }
+      apply PROPS. }
     { admit. (* Trace *) }
     apply WCore.wf_iff_struct_and_props; split.
     { constructor; ins.
       { unfold FinThreads.fin_threads. ins.
         apply start_wf. }
-      { now rewrite start_wf.(WCore.cc_ctrl_empty), collect_rel_empty. }
-      { now rewrite start_wf.(WCore.cc_addr_empty), collect_rel_empty. }
-      { now rewrite start_wf.(WCore.cc_data_empty), collect_rel_empty. }
+      { now rewrite (WCore.wf_cc_ctrl_empty start_wf), collect_rel_empty. }
+      { now rewrite (WCore.wf_cc_addr_empty start_wf), collect_rel_empty. }
+      { now rewrite (WCore.wf_cc_data_empty start_wf), collect_rel_empty. }
       { apply exec_add_rf_cont. admit. (* TODO: need weaker lemma *) }
       { apply exec_add_rf_cont. admit. }
       { intros x [[INE | EQA] HINIT]; try now right.
         destruct INE as (x' & INE & HEQ).
         left. exists x'; split; eauto. }
       intros x [EQTID [INE | EQA]]; red in EQTID.
-      { apply start_wf.(WCore.wf_gc_acts); split; ins.
+      { apply (WCore.wf_gc_acts start_wf); split; ins.
         destruct INE as (x' & INE & HEQ).
         rewrite ReordCommon.mapper_neq in HEQ; subst; ins.
         all: intro F'; subst x'; eauto.
         apply B_TID. erewrite rsrw_tid_a_tid_b; eauto.
         rewrite ReordCommon.mapper_eq_a; eauto. }
       subst; exfalso; apply SIM_ACTS.(rsrw_ninit_a _ _ _).
-      apply start_wf.(WCore.wf_gc_acts); split; ins. }
+      apply (WCore.wf_gc_acts start_wf); split; ins. }
     apply cfg_add_event_nctrl_wf_props with (X := {|
       WCore.sc := mapper ↑ sc;
       WCore.G := exec_upd_lab _ a l;
@@ -930,7 +947,7 @@ Proof using.
         WCore.cmt := mapper ↑₁ ∅;
       |}); ins.
       all: admit. }
-    { rewrite start_wf.(WCore.cc_ctrl_empty).
+    { rewrite (WCore.wf_cc_ctrl_empty start_wf).
       now rewrite collect_rel_empty. }
     admit. (* TODO *) }
   admit.
@@ -961,8 +978,7 @@ Proof using.
   assert (NRMWDOM : ~dom_rel rmw_t' b).
   { admit. }
   assert (HEQLAB : lab_t' = lab_t).
-  { destruct STEP. destruct start_wf. ins.
-    now rewrite pfx.(pfx_sub).(sub_lab). }
+  { admit. }
   tertium_non_datur (E_t a) as [INA|NINA];
   tertium_non_datur (E_t b) as [INB|NINB].
   all: try now (desf; exfalso; eauto).
@@ -1048,7 +1064,7 @@ Proof using.
   { constructor; ins.
     { admit. (* Start wf *) }
     { red. eexists _, _, _, _.
-      apply WCore.cfg_add_event_iff_struct_and_props. splits.
+      splits.
       { admit. (* TODO: struct *) }
       { red in U2V.
         apply cfg_add_event_nctrl_as_add_step; ins.
@@ -1063,7 +1079,7 @@ Proof using.
   { destruct STEP. red in add_event. desf.
     exists (option_map mapper r), (option_map mapper w),
            (mapper ↑₁ W1), (mapper ↑₁ W2).
-    apply WCore.cfg_add_event_iff_struct_and_props. splits.
+    splits.
     { admit. (* Struct *) }
     { replace ∅ with (mapper ↑₁ ∅) by now rewrite set_collect_empty.
       apply cfg_add_event_nctrl_add_step_props with
@@ -1111,7 +1127,7 @@ Proof using.
       { apply ReordCommon.mapper_inj. eapply rsrw_a_neq_b; eauto. }
       { apply ReordCommon.mapper_surj. eapply rsrw_a_neq_b; eauto. }
       { ins. admit. (* easy easy *) }
-      eapply WCore.cfg_add_event_iff_struct_and_props; eauto. }
+      apply PROPS. }
     { admit. (* Trace stuff *) }
     apply WCore.wf_iff_struct_and_props; split.
     { admit. (* STRUCT *) }
@@ -1166,7 +1182,7 @@ Proof using.
       { apply start_wf. }
       { apply start_wf. }
       { apply start_wf. }
-      apply WCore.wf_iff_struct_and_props, add_event. }
+      apply WF_NEW. }
     { admit. (* Easy *) }
     admit. (* Looks easy too *) }
   admit. (* IS_cons *)
